updateMonadCoqAsts.sh
@@ -12,5 +12,5 @@ CPP2V=../_build/install/default/bin/cpp2v
 mkdir -p $DST
 cp build/compile_commands.json ./ # cpp2v extracts the compile flags from here and passes the same to the clang AST visitor library
 $CPP2V  ./libs/execution/src/monad/execution/execute_block.cpp --no-elaborate -o $(pwd)/$DST/exb.v # --templates exb_templates.v
-$CPP2V  ./libs/execution/src/monad/execution/execute_transaction.cpp --no-elaborate -o $(pwd)/$DST/ext.v #-templates $(pwd)/$DST/ext_templates.v
-$CPP2V  ./libs/execution/src/monad/state2/block_state.cpp --no-elaborate -o $(pwd)/$DST/block_state_cpp.v #-templates $(pwd)/$DST/block_state_templates.v
+#$CPP2V  ./libs/execution/src/monad/execution/execute_transaction.cpp --no-elaborate -o $(pwd)/$DST/ext.v #-templates $(pwd)/$DST/ext_templates.v
+#CPP2V  ./libs/execution/src/monad/state2/block_state.cpp --no-elaborate -o $(pwd)/$DST/block_state_cpp.v #-templates $(pwd)/$DST/block_state_templates.v
